Task 1.
 i.  f / g (x) = f(x) / g(x)
    (2x + 1 / x<sup>2</sup>) / (3x-1 / (x -1)<sup>3</sup>)
    (2x + 1 / x<sup>2</sup>) * ((x-1)<sup>3</sup> / 3x-1)
	(2x + 1) (x-1)<sup>3</sup>  / (x<sup>2</sup> ) (3x -1)
	 (2x + 1) ((x-1)(x-1)(x-1)) /  (x<sup>2</sup> ) (3x -1)
	 (2x + 1)(x<sup>2</sup> - 2x + 1(x-1)) / (x<sup>2</sup> ) (3x -1)
	 (2x+1)(x<sup>3</sup>- 2x<sup>2</sup> + x - x<sup>2</sup> +2x-1) / (x<sup>2</sup> ) (3x -1)
	 (2x + 1)(x<sup>3</sup>-2x<sup>2</sup> - x<sup>2</sup> +x +2x - 1) / (x<sup>2</sup> ) (3x -1)
	 (2x+ 1)(x<sup>3</sup> - 3x<sup>2</sup> + 3x - 1) / 3x<sup>2</sup> - x<sup>2</sup> 
	  (2x+ 1)(x<sup>3</sup> - 3x<sup>2</sup> + 3x - 1) / 4x
    

 fog = f(g(x))
    
    
       




Task 2

y = sqrt(20c + 15 / 15c + 16)
y<sup>2</sup>  = 20c + 15 / 15c + 16

y<sup>2</sup> (15c + 16) = 20c + 15
15y<sup>2</sup> c + 16y<sup>2</sup>  = 20c +15
15y<sup>2</sup> c - 20c = 15 + 16<sup>2</sup>  y
c(15y<sup>2</sup> - 20) = 15 + 16<sup>2</sup>  y
c = 15 + 16<sup>2</sup>  y / 15y<sup>2</sup> - 20