Task 1
i x + y + z  = 25
20x - 3(y + z) = 0
20x -3y - 3z = 0
5(x + y + z) = 125
5x + 5y + 5z = 125

x + y + z = 25
20x - 3y - 3z = 0
5x + 5y + 57 = 125

ii. 

iii. x + y + z = 25
20x - 3y - 3z = 0
5x + 5y + 57 = 125

x + y + z = 25 
20x - 3y - 3z = 0

-20x - 20y -20z = 25
20x -3y -3z = 0


Task 2
x - y + z = 4
5x - y + z = 6
3x - y + 5z = 5

1  - 1    1   4
5  - 1    1   6
3  - 1    5   5


5R1 - R2 = R2 ->  1     -1    1    4
                0     4    -4   -14
                3     -1   5     5

3R1 - R3 =  R3 ->   1    -1     1   4
                0     4    -4   -14
                0    2      2      -24

1 / 4R2 = R2  ->      1     -1     1       4
				0     1     -1   -7/2
				0     2       2      -2

R3 - 2R2 = R3   -> 1     -1     1       4
				0     1     -1   -7/2
				0     0      4      0

4z = 0
z = 0

y - z = -7/2

y - 0 =  -7 / 2

y  = -7 /2 

x - y + z = 4

x - (-7/2) + 0 = 4
x + 7/2 = 4 
x = 4 -7/2
x = 4/1 - 7 /2
x = 8 - 7  / 2
x = 1/2

(1/2, -7/2, 0)

Task 3 
x + y = 4
x^2 - 2xy - 3 = 0

make x the subject of the formula
x + y = 4
y = 4 -x

substitute x in equation 2
x ^ 2 - 2xy - 3 = 0
x^2 - 2x(4 - x) - 3 = 0
x^2 - 8x + 2x^2 - 3 = 0
x^2 + 2x^2 -8x - 3 = 0
3x^2 - 8x - 3 = 0

x = -b ± sqrt(b^2−4ac) / 2a

a = 3,  b = -8, c = -3

x = -(-8) ± sqrt(-8 ^ 2 - 4(3)(-3)) / 2(3)
x = 8 ± sqrt(64  + 36 ) / 6
x = 8 ± sqrt(100) /6
x = 8 ± 10 /6

x = 8 + 10 / 6  or  x = 8 - 10 / 6
x = 18 / 6   or x = -2 /6
x = 3 or -1/3

y = 4 - x

y = 4 - 3 or y = 4 + 1/3

 y = 1 or y = 4 / 1 + 1 / 3
 y = 1 or y = 12 + 1 /3
 y = 1 or y = 13 / 3

x = 3, y = 1
x = -1/3, y = 13 / 3