Task 1
i. Exponential functions are functions are functions that grow or decay at a rate proportional to their current value while logarithmic functions are functions which are an inverse operation of an exponential function.

a logarithmic function is an inverse operation of an exponential function.

f(x) = ab<sup>x</sup> 
f(x) = it is the output of the exponential function
a = initial value
b = the base value which is a constant greater than zero and not equal to one
x = the input  value.

f(x) = log<sub>b</sub> (x)
f(x) = it is the output of the logarithmic function
log<sub>b</sub> = it denotes the logarithmic function with base b
b = it denotes the base of the function
x = it is the input value.

ii. 
iii. A function has exponential growth if there is percentage increase in the original value overtime. 

iv. An exponential function grow much faster because in exponential function as the input increases the output of the function increases rapidly while in logarithmic functions as the input increases the rate at which it grows diminishes 


Task 2
 i log<sub>6</sub> (216<sup>x</sup> / 1296<sup>x</sup>) log<sub>x</sub> 6
log<sub>6</sub>216<sup>x</sup> - log<sub>6</sub>1296<sup>x</sup>  (log<sub>x</sub> 6)
xlog<sub>6</sub>216 - xlog<sub>6</sub>1296 (log<sub>x</sub> 6)
log<sub>6</sub> 216 = log<sub>6</sub> (6)<sup>3</sup>  = 3
log<sub>6</sub> 1296 = log<sub>6</sub> (6)<sup>4</sup>  = 4

3x - 4x  (log<sub>x</sub> 6)

ii. log<sub>e</sub>(x + 1)<sup>2</sup> + log<sub>e</sub>(2x - 1)<sup>3</sup>- log<sub>e</sub>(x)<sup>2</sup> - log<sub>e</sub>(2x - 1)<sup>4</sup> + 6log<sub>e</sub>(x + 1)
log<sub>e</sub> (x + 1)<sup>2</sup> (2x - 1)<sup>3</sup>  - log<sub>e</sub>(x)<sup>2</sup> - log<sub>e</sub>(2x - 1)<sup>4</sup> + 6log<sub>e</sub>(x + 1)
log<sub>e</sub> ((x + 1)<sup>2</sup> (2x - 1)<sup>3</sup> /  x<sup>2</sup> ) - log<sub>e</sub>(2x - 1)<sup>4</sup> + log<sub>e</sub>(x + 1)<sup>6</sup> 
log<sub>e</sub> ((x + 1)<sup>2</sup> (2x - 1)<sup>3</sup> /  x<sup>2</sup> ) - log<sub>e</sub> ((2x - 1)<sup>4</sup> (x + 1)<sup>6</sup> )
log<sub>e</sub> ((x + 1)<sup>2</sup> (2x - 1)<sup>3</sup> /  x<sup>2</sup> ) / ((2x - 1)<sup>4</sup> (x + 1)<sup>6</sup> )

iii. 10<sub>e</sub>(2x - 3) = 15<sub>e</sub> (5x - 7)
10<sub>e</sub> = 1
e(2x - 3) = (e + 5) (5x - 7)
2ex−3e=5ex−7e+25x−35
2ex - 5ex - 25x = -7e + 3e - 35
-3ex- 25x = -4e - 35
x(-3e - 15) = -4e - 35
x = -4e - 35 / -3e - 15

Task 3
i. N(x) = N<sub>0</sub>(1 + r)<sup>x</sup> 
N(x) = 232.26(1 + 0.02)<sup>x</sup> 
N(x) = 232.26(1.02)<sup>x</sup> 

2019
N(1) = 232.26(1.02)<sup>1</sup> 
= 232.26(1.02)
= 236.844

2020
N(2) = 232.26(1)<sup>2</sup> 
= 232.26(1.0404)
= 241.643

2021
N(3) = 232.26(1.02)<sup>3</sup> 
= 232.26(1.061208)
= 246.4762

2022
N(4) = 232.26(1.02)<sup>4</sup> 
= 232.26(1.08243216)
= 251.406

2023
N(5) = 232.26(1.02)<sup>5</sup> 
= 232.26(1.126162419264)
= 261.562

2018       2019            2020            2021             2022            2023
232.26    236.844       241.643       246.4762      251.406         261.562


ii. 
N(x) = N<sub>0</sub>(1 + r)<sup>x</sup> 
N<sub>0</sub> = initial value
r = growth rate in %
x = number of years after 2018


iii N(20) = N<sub>0</sub>(1 + r)<sup>20</sup> 
232.26(1 + 0.02)<sup>20</sup> 
232.26(1.02)<sup>20</sup> 
232.26(1.485947)
345.1261

iv
