When we combine two relationships

We can combine two functions using algebraic operations.
for two functions f(x) and g(x) with real numbers as their output, we define the new function as the following:

(f + g)(x) = f(x) + g(x)
(f - g)(x) = f(x) - g(x)
(f * g)(x) = f(x) *  g(x)
(f / g)(x) = f(x) / g(x)

(fg)(x) and (f-g)x, where f(x) = x - 1 and g(x) = x ^ 2 - 1

(fg)(x) = f(x) * g(x)
        x- 1 * ( x^2 - 1)
        x^3 + 1
(f - g)(x) = f(x) - g(x)
		 x -1 - (x^2 -1)
		 x - 1 - x^2 +1
		 x - x^2
		 x(1 - x)




The process of combining functions by making the output of one function the input of another function is known as combinations of functions.
Note: the range of the inside function(the first to be evaluated) must be within the domain of the outside function


## Inverse Function
 An inverse function is a function whose output is the input of the original function and its input is the  output of the original function